named_api/API/core.v
@@ -127,6 +127,7 @@ Definition weaken_context : state -> context -> context :=
 Record one_param_env : Type := mk_one_param_env
 { ep_kname          : kername ;
   ep_nb_uparams     : nat ;
+  ep_type_uparams   : list term ;
   ep_strpos_uparams : list bool ;
   ep_cparam_kname   : kername ;
   ep_fdt_kname      : kername;
