named_api/Functoriality/functoriality.v
@@ -143,7 +143,7 @@ Fixpoint make_func_call (s : state) (key_arg : key) (ty : term) {struct ty} : te
       let* s _ key_locals _ := closure_context_sep tLambda s (Some "locals") loc in
       mkApp (mkApps (geti_term s key_fixs pos_indb) (local_nuparams ++ local_indices))
             (mkApps (get_term  s key_arg) (get_terms s key_locals))
-  | SPArgIsNested xp pos_indb loc local_uparams local_nuparams_indices =>
+  | SPArgIsNested xp pos_indb loc local_uparams local_nuparams_indices _ =>
       let compute_nested_rc (x : term) (s s : state) : term :=
         let* s key_farg := mk_tLambda s (Some "rec_arg") (mkBindAnn nAnon Relevant) x in
         make_func_call s key_farg (lift0 1 x)
