named_api/UnitTests/t07_nested_types.v
@@ -322,7 +322,7 @@ Unset Elimination Schemes.
 Inductive typing A B (n : nat) (a : A) (b : B) : Type :=
 | typ_nil  : typing A B n a b
 | typ_cons : forall (lA : list A) (lB : list B),
-             All2i A B (typing A B) n lA lB -> typing A B n a b.
+             nesting_param.All2i A B (typing A B) n lA lB -> typing A B n a b.
 
 (* It means correcting the computation of uparams of Coq  *)
 Definition typing_ind A B (P : forall n a b, typing A B n a b -> Prop)
@@ -345,7 +345,7 @@ Inductive typing_param1 A B : forall n a b, typing A B n a b -> Prop :=
                     forall x, All2i_param1 A B (typing A B) (fun n a b x => typing_param1 A B n a b x) n lA lB x ->
                     typing_param1 A B n a b (typ_cons A B n a b lA lB x).
 
-(* MetaCoq Run (tmMsg "11/15 typing"). *)
+MetaCoq Run (tmMsg "15/15 typing").
 Redirect "named_api/UnitTests/tests/07_15_typing_coq" MetaCoq Run (print_rec "typing").
 Redirect "named_api/UnitTests/tests/07_15_typing_gen" MetaCoq Run (generate Ep (@typing)).
 
